matching-logic/src/DerivedOperators.v
@@ -118,6 +118,56 @@ Module Syntax.
       intros. simpl. do 2 rewrite andb_true_r. auto.
     Qed.
     
+    Lemma bevar_subst_not ψ (wfψ : well_formed_closed ψ) x ϕ :
+      bevar_subst (patt_not ϕ) ψ x = patt_not (bevar_subst ϕ ψ x).
+    Proof. simpl. unfold patt_not. reflexivity. Qed.
+
+    Lemma bevar_subst_or ψ (wfψ : well_formed_closed ψ) x ϕ₁ ϕ₂ :
+      bevar_subst (patt_or ϕ₁ ϕ₂) ψ x = patt_or (bevar_subst ϕ₁ ψ x) (bevar_subst ϕ₂ ψ x).
+    Proof. simpl. unfold patt_or. unfold patt_not. reflexivity. Qed.
+
+    Lemma bevar_subst_and ψ (wfψ : well_formed_closed ψ) x ϕ₁ ϕ₂ :
+      bevar_subst (patt_and ϕ₁ ϕ₂) ψ x = patt_and (bevar_subst ϕ₁ ψ x) (bevar_subst ϕ₂ ψ x).
+    Proof. simpl. unfold patt_and. unfold patt_not. reflexivity. Qed.
+
+    Lemma bevar_subst_iff ψ (wfψ : well_formed_closed ψ) x ϕ₁ ϕ₂ :
+      bevar_subst (patt_iff ϕ₁ ϕ₂) ψ x = patt_iff (bevar_subst ϕ₁ ψ x) (bevar_subst ϕ₂ ψ x).
+    Proof. simpl. unfold patt_iff. unfold patt_and. unfold patt_not. reflexivity. Qed.
+
+    Lemma bevar_subst_top ψ (wfψ : well_formed_closed ψ) x : bevar_subst patt_top ψ x = patt_top.
+    Proof. simpl. unfold patt_top. unfold patt_not. reflexivity. Qed.
+
+    Lemma bevar_subst_forall ψ (wfψ : well_formed_closed ψ) x ϕ :
+      bevar_subst (patt_forall ϕ) ψ x = patt_forall (bevar_subst ϕ ψ (S x)).
+    Proof. simpl. unfold patt_forall. unfold patt_not. reflexivity. Qed.
+
+    (* TODO: bevar_subst_nu *)
+
+    Lemma bsvar_subst_not ψ (wfψ : well_formed_closed ψ) x ϕ :
+      bsvar_subst (patt_not ϕ) ψ x = patt_not (bsvar_subst ϕ ψ x).
+    Proof. simpl. unfold patt_not. reflexivity. Qed.
+
+    Lemma bsvar_subst_or ψ (wfψ : well_formed_closed ψ) x ϕ₁ ϕ₂ :
+      bsvar_subst (patt_or ϕ₁ ϕ₂) ψ x = patt_or (bsvar_subst ϕ₁ ψ x) (bsvar_subst ϕ₂ ψ x).
+    Proof. simpl. unfold patt_or. unfold patt_not. reflexivity. Qed.
+
+    Lemma bsvar_subst_and ψ (wfψ : well_formed_closed ψ) x ϕ₁ ϕ₂ :
+      bsvar_subst (patt_and ϕ₁ ϕ₂) ψ x = patt_and (bsvar_subst ϕ₁ ψ x) (bsvar_subst ϕ₂ ψ x).
+    Proof. simpl. unfold patt_and. unfold patt_not. reflexivity. Qed.
+
+    Lemma bsvar_subst_iff ψ (wfψ : well_formed_closed ψ) x ϕ₁ ϕ₂ :
+      bsvar_subst (patt_iff ϕ₁ ϕ₂) ψ x = patt_iff (bsvar_subst ϕ₁ ψ x) (bsvar_subst ϕ₂ ψ x).
+    Proof. simpl. unfold patt_iff. unfold patt_and. unfold patt_not. reflexivity. Qed.
+
+    Lemma bsvar_subst_top ψ (wfψ : well_formed_closed ψ) x : bsvar_subst patt_top ψ x = patt_top.
+    Proof. simpl. unfold patt_top. unfold patt_not. reflexivity. Qed.
+
+    Lemma bsvar_subst_forall ψ (wfψ : well_formed_closed ψ) x ϕ :
+      bsvar_subst (patt_forall ϕ) ψ x = patt_forall (bsvar_subst ϕ ψ x).
+    Proof. simpl. unfold patt_forall. unfold patt_not. reflexivity. Qed.
+
+    (* ******* *)
+
     Lemma evar_open_not k x ϕ : evar_open k x (patt_not ϕ) = patt_not (evar_open k x ϕ).
     Proof. simpl. unfold patt_not. reflexivity. Qed.
 
@@ -162,43 +212,43 @@ Module Syntax.
     #[global]
      Instance Unary_not : Unary patt_not :=
       {|
-      unary_evar_open := evar_open_not ;
-      unary_svar_open := svar_open_not ;
+      unary_bevar_subst := bevar_subst_not ;
+      unary_bsvar_subst := bsvar_subst_not ;
       |}.
 
     #[global]
      Instance NVNullary_top : NVNullary patt_top :=
       {|
-      nvnullary_evar_open := evar_open_top ;
-      nvnullary_svar_open := svar_open_top ;
+      nvnullary_bevar_subst := bevar_subst_top ;
+      nvnullary_bsvar_subst := bsvar_subst_top ;
       |}.
 
     #[global]
      Instance Binary_or : Binary patt_or :=
       {|
-      binary_evar_open := evar_open_or ;
-      binary_svar_open := svar_open_or ;
+      binary_bevar_subst := bevar_subst_or ;
+      binary_bsvar_subst := bsvar_subst_or ;
       |}.
 
     #[global]
      Instance Binary_and : Binary patt_and :=
       {|
-      binary_evar_open := evar_open_and ;
-      binary_svar_open := svar_open_and ;
+      binary_bevar_subst := bevar_subst_and ;
+      binary_bsvar_subst := bsvar_subst_and ;
       |}.
 
     #[global]
      Instance Binary_iff : Binary patt_iff :=
       {|
-      binary_evar_open := evar_open_iff ;
-      binary_svar_open := svar_open_iff ;
+      binary_bevar_subst := bevar_subst_iff ;
+      binary_bsvar_subst := bsvar_subst_iff ;
       |}.
 
     #[global]
      Instance EBinder_forall : EBinder patt_forall _ _ :=
       {|
-      ebinder_evar_open := evar_open_forall ;
-      ebinder_svar_open := svar_open_forall ;
+      ebinder_bevar_subst := bevar_subst_forall ;
+      ebinder_bsvar_subst := bsvar_subst_forall ;
       |}.
   
   
@@ -383,7 +433,8 @@ Module Semantics.
         unfold patt_forall.
         apply M_predicate_not.
         apply M_predicate_exists.
-        rewrite !simpl_evar_open.
+        unfold evar_open.
+        repeat (rewrite simpl_bevar_subst';[reflexivity|]).
         apply M_predicate_not.
         subst x.
         simpl.        
@@ -488,7 +539,8 @@ Module Semantics.
         }
 
         rewrite -> Hfr. subst x.
-        rewrite !simpl_evar_open.
+        unfold evar_open.
+        simpl_bevar_subst.
         split; intros H'.
         - intros m.
           specialize (H' m).
